theories/simulations/msim/ISimFacts.v
@@ -1,468 +1,31 @@
 From CRIS.common Require Import Common ConcRA StatePredicate.
-From CRIS.modules Require Import LMod Mod SMod Sp.
-From CRIS.simulations.msim Require Import MSim MSimFacts
-  MSimCommon ISim TacticsCommon ITactics.
+From CRIS.modules Require Import Mod.
+From CRIS.simulations.msim Require Import MSimCommon ISim.
+From CRIS.simulations.msim Require Export ISimExtendCtx ISimHorComp
+  ISimFrame ISimRefl.
 From iris.proofmode Require Import proofmode.
-From stdpp Require Import base list.
 
-Section ISIM_FRAME.
-  Context `{!crisG Γ Σ α β τ _S _I}.
-  Context `{!stateGS Σ}.
-
-  Lemma isim_ist_frame ctx Ist P Rs Rt RR fl_src fl_tgt
-      ps pt (i_s : itree crisE Rs) (i_t : itree crisE Rt) :
-    P ∗ isim ctx fl_src fl_tgt Ist ibot RR ps pt i_s i_t ⊢
-    isim ctx fl_src fl_tgt
-      (P ∗ Ist)%I ibot (λ x y, P ∗ RR x y) ps pt i_s i_t.
-  Proof using.
-    eapply entails_pointwise. intros res VALID H.
-    eapply isim_final.
-    eapply Own_split in H as
-      [rP [rSIM [EQ [HP HSIM]]]]; eauto.
-    eapply isim_init in HSIM; et.
-    gfinal. right.
-    eapply paco8_mon; [eapply msim_ist_frame|]; ss.
-    - ginit. eapply gpaco8_mon; eauto using iunlift_ibot.
-    - rewrite EQ Own_op HP. et.
-  Qed.
-End ISIM_FRAME.
-
-Section STATE_EQ.
-  Context {Σ : GRA}.
-
-  Definition state_eq (S : gset string) (STATE : stateGS Σ) : iProp Σ :=
-    ∃ st_src st_tgt : gmap key (option Any.t),
-      ⌜state_slice S st_src = state_slice S st_tgt⌝ ∗
-      state_init_src S st_src STATE ∗ state_init_tgt S st_tgt STATE.
-
-  Definition IstEq (M : Mod.t) : stateGS Σ → iProp Σ :=
-    state_eq (list_to_set (Mod.scopes M)).
-
-  Lemma state_eq_acc `{STATE : !stateGS Σ} S k (IN : k.1 ∈ S) :
-    state_eq S STATE ⊢
-      ∃ ov, state_cell_src k ov ∗ state_cell_tgt k ov ∗
-        (∀ ov', ⌜state_cell_transition ov ov'⌝ -∗
-          state_cell_src k ov' ∗ state_cell_tgt k ov' -∗
-          state_eq S STATE).
-  Proof.
-    rewrite /state_eq /=. iIntros "EQ".
-    iDestruct "EQ" as (st_src st_tgt) "(%EQ & SRC & TGT)".
-    iPoseProof (state_init_src_acc S st_src k IN with "SRC") as
-      (ov_src) "(%Hsrc & SRC & CLOSESRC)".
-    iPoseProof (state_init_tgt_acc S st_tgt k IN with "TGT") as
-      (ov_tgt) "(%Htgt & TGT & CLOSETGT)".
-    assert (Hov : ov_src = ov_tgt).
-    { rewrite Hsrc Htgt.
-      pose proof (f_equal (fun st => st !! k) EQ) as EQk.
-      rewrite (state_slice_lookup_in S st_src k IN)
-        (state_slice_lookup_in S st_tgt k IN) in EQk.
-      exact EQk. }
-    clear Htgt. subst ov_tgt.
-    iExists ov_src. iFrame "SRC TGT".
-    iIntros (ov') "%TRANS [SRC TGT]".
-    iExists (set_state_cell k ov' st_src),
-      (set_state_cell k ov' st_tgt).
-    iSplit.
-    { iPureIntro.
-      by apply state_slice_set_state_cell_eq. }
-    iSplitL "SRC CLOSESRC".
-    - iApply ("CLOSESRC" $! ov' with "[] SRC"). done.
-    - iApply ("CLOSETGT" $! ov' with "[] TGT"). done.
-  Qed.
-
-  Lemma state_eq_put `{STATE : !stateGS Σ} S k v' (IN : k.1 ∈ S) :
-    state_eq S STATE ⊢
-      ∃ ov, state_cell_src k ov ∗ state_cell_tgt k ov ∗
-        ((k ↦src v' ∗ k ↦tgt v') -∗ state_eq S STATE).
-  Proof.
-    iIntros "EQ".
-    iPoseProof (state_eq_acc S k IN with "EQ") as
-      (ov) "(SRC & TGT & CLOSE)".
-    iExists ov. iFrame "SRC TGT". iIntros "[SRC TGT]".
-    iApply ("CLOSE" $! (Some v') with "[] [SRC TGT]").
-    - iPureIntro. right. done.
-    - rewrite /state_cell_src /state_cell_tgt /=. iFrame.
-  Qed.
-
-  Lemma state_eq_get `{STATE : !stateGS Σ} S k (IN : k.1 ∈ S) :
-    state_eq S STATE ⊢
-      ∃ ov, state_cell_src k ov ∗ state_cell_tgt k ov ∗
-        ((state_cell_src k ov ∗ state_cell_tgt k ov) -∗
-          state_eq S STATE).
-  Proof.
-    iIntros "EQ".
-    iPoseProof (state_eq_acc S k IN with "EQ") as
-      (ov) "(SRC & TGT & CLOSE)".
-    iExists ov. iFrame "SRC TGT". iIntros "ST".
-    iApply ("CLOSE" $! ov with "[] ST").
-    iPureIntro. left. done.
-  Qed.
-
-  Lemma state_eq_init `{STATE : !stateGS Σ} S st_src st_tgt
-      (EQ : state_slice S st_src = state_slice S st_tgt) :
-    state_init_src S st_src STATE -∗
-    state_init_tgt S st_tgt STATE -∗
-    state_eq S STATE.
-  Proof.
-    iIntros "SRC TGT". iExists st_src, st_tgt. iFrame. done.
-  Qed.
-
-  Lemma state_eq_init_same `{STATE : !stateGS Σ} S st :
-    state_init_src S st STATE -∗
-    state_init_tgt S st STATE -∗
-    state_eq S STATE.
-  Proof.
-    iApply state_eq_init. done.
-  Qed.
-End STATE_EQ.
-
-Section ISIM_REFL.
-  Context `{!crisG Γ Σ α β τ _S _I}.
-  Context `{STATE : !stateGS Σ}.
-
-  (* Reflexivity of the isim relation *)
-  Lemma isim_refl g ctx (Ist : iProp Σ) fl_src fl_tgt msk ps pt {R}
-      (it : itree crisE R) :
-    (∀ k v', msk _ (subevent _ (SPut k v')) = true →
-      Ist ⊢ ∃ ov, state_cell_src k ov ∗ state_cell_tgt k ov ∗
-        ((k ↦src v' ∗ k ↦tgt v') -∗ Ist)) →
-    (∀ k, msk _ (subevent _ (SGet k)) = true →
-      Ist ⊢ ∃ ov, state_cell_src k ov ∗ state_cell_tgt k ov ∗
-        ((state_cell_src k ov ∗ state_cell_tgt k ov) -∗ Ist)) →
-    Ist ⊢
-    isim ctx fl_src fl_tgt Ist g (ist_with_eq Ist) ps pt
-      (SB.sandbox msk it) (SB.sandbox msk it).
-  Proof using.
-    intros Hset Hget.
-    revert it. combine_quant ps. combine_quant pt.
-    eapply isim_coind. intros g0 _ CIH [pt [ps it]].
-    destruct_quant CIH. iIntros "IST /=".
-    assert (CASE := case_itrH it); des; subst.
-    - istep. iFrame. done.
-    - istep_s. istep_t. iby_coind CIH; eauto.
-    - cNormT; cNormS. des_if.
-      { istep_s. iforce_t; iFrame "ASM". cNormT. iby_coind CIH. eauto. }
-      { istep_s; ss. }
-    - cNormT; cNormS. des_if.
-      { istep_s. iforce_t; iFrame "ASM". cNormT. iby_coind CIH. eauto. }
-      { istep_s; ss. }
-    - cNormT; cNormS. des_if.
-      { istep_t. iforce_s; iFrame. cNormS. iby_coind CIH. eauto. }
-      { istep_s; ss. }
-    - depdes c.
-      { cNormT; cNormS. des_if.
-        { icall "IST" as (?) "IST"; et. iby_coind CIH; eauto. }
-        { isteps_s; ss. }
-      }
-      { cNormT; cNormS. des_if.
-        { istep. iby_coind CIH; done. }
-        { isteps_s. ss. }
-      }
-      { cNormS; cNormT. des_if.
-        { iyield "IST" "IST". iby_coind CIH. eauto. }
-        { isteps_s. ss. }
-      }
-      { cNormS; cNormT. des_if.
-        { istep. iby_coind CIH. eauto. }
-        { isteps_s. ss. }
-      }
-    - depdes s.
-      { cNormT; cNormS.
-        rewrite ?resum_to_subevent ?subevent_subevent.
-        specialize (Hset k v); destruct (msk _ _) eqn:Hmsk;
-          [cNormS; cNormT|istep_s; ss].
-        iPoseProof (Hset eq_refl with "IST") as
-          (ov) "(SRC & TGT & CLOSE)".
-        destruct ov as [v0|].
-        - iEval (rewrite /state_cell_src /state_cell_tgt /=) in "SRC TGT".
-          iApply isim_sput_src. iFrame "SRC". iIntros "SRC".
-          iApply isim_sput_tgt. iFrame "TGT". iIntros "TGT".
-          iby_coind CIH. iApply ("CLOSE" with "[$SRC $TGT]").
-        - iEval (rewrite /state_cell_src /state_cell_tgt /=) in "SRC TGT".
-          iApply isim_sput_src_uninit. iFrame "SRC". iIntros "SRC".
-          iApply isim_sput_tgt_uninit. iFrame "TGT". iIntros "TGT".
-          iby_coind CIH. iApply ("CLOSE" with "[$SRC $TGT]").
-      }
-      { cNormT; cNormS.
-        rewrite ?resum_to_subevent ?subevent_subevent.
-        specialize (Hget k); destruct (msk _ _) eqn:Hmsk;
-          [cNormS; cNormT|istep_s; ss].
-        iPoseProof (Hget eq_refl with "IST") as
-          (ov) "(SRC & TGT & CLOSE)".
-        destruct ov as [v|].
-        - iEval (rewrite /state_cell_src /state_cell_tgt /=) in "SRC TGT".
-          iApply isim_sget_src. iFrame "SRC". iIntros "SRC".
-          iApply isim_sget_tgt. iFrame "TGT". iIntros "TGT".
-          iby_coind CIH.
-          iApply ("CLOSE" with "[$SRC $TGT]").
-        - iEval (rewrite /state_cell_src /state_cell_tgt /=) in "SRC TGT".
-          iApply isim_sget_src_uninit. iFrame "SRC". iIntros "SRC".
-          iApply isim_sget_tgt_uninit. iFrame "TGT". iIntros "TGT".
-          iby_coind CIH.
-          iApply ("CLOSE" with "[$SRC $TGT]").
-      }
-    - destruct e.
-      + cNormT; cNormS. des_if; [cNormS; cNormT|istep_s; ss].
-        istep_t. iforce_s. cNormS; cNormT; iby_coind CIH; eauto.
-      + cNormT; cNormS. des_if; [cNormS; cNormT|istep_s; ss].
-        istep_s. iforce_t. cNormS; cNormT; iby_coind CIH; eauto.
-      + cNormT; cNormS. des_if; [cNormS; cNormT|istep_s; ss].
-        istep. cNormS; cNormT; iby_coind CIH; eauto.
-  Qed.
-
-  Lemma isim_reflL
-      (ctx : contextuality) (fl_src fl_tgt : gmap fname (option fbody))
-      (msk : emask) (EqL Ist : iProp Σ) itr :
-    (∀ k v', msk _ (subevent _ (SPut k v')) = true →
-      EqL ⊢ ∃ ov, state_cell_src k ov ∗ state_cell_tgt k ov ∗
-        ((k ↦src v' ∗ k ↦tgt v') -∗ EqL)) →
-    (∀ k, msk _ (subevent _ (SGet k)) = true →
-      EqL ⊢ ∃ ov, state_cell_src k ov ∗ state_cell_tgt k ov ∗
-        ((state_cell_src k ov ∗ state_cell_tgt k ov) -∗ EqL)) →
-    ⊢ isim_fsem fl_src fl_tgt (EqL ∗ Ist)%I ctx
-        (SB.sandbox_body (msk, itr)) (SB.sandbox_body (msk, itr)).
-  Proof using.
-    intros Hset Hget. rewrite /isim_fsem.
-    iIntros "!#" (arg) "[E I] _".
-    rewrite /SB.sandbox_body /=. iApply isim_refl.
-    - intros k v' Hmsk. iIntros "[E I]".
-      iPoseProof (Hset k v' Hmsk with "E") as
-        (ov) "(SRC & TGT & CLOSE)".
-      iExists ov. iFrame "SRC TGT". iIntros "[SRC TGT]".
-      iSplitR "I"; last done. iApply ("CLOSE" with "[$SRC $TGT]").
-    - intros k Hmsk. iIntros "[E I]".
-      iPoseProof (Hget k Hmsk with "E") as
-        (ov) "(SRC & TGT & CLOSE)".
-      iExists ov. iFrame "SRC TGT". iIntros "[SRC TGT]".
-      iSplitR "I"; last done. iApply ("CLOSE" with "[$SRC $TGT]").
-    - iFrame.
-  Qed.
-
-  Lemma isim_reflR
-      (ctx : contextuality) (fl_src fl_tgt : gmap fname (option fbody))
-      (msk : emask) (Ist EqR : iProp Σ) itr :
-    (∀ k v', msk _ (subevent _ (SPut k v')) = true →
-      EqR ⊢ ∃ ov, state_cell_src k ov ∗ state_cell_tgt k ov ∗
-        ((k ↦src v' ∗ k ↦tgt v') -∗ EqR)) →
-    (∀ k, msk _ (subevent _ (SGet k)) = true →
-      EqR ⊢ ∃ ov, state_cell_src k ov ∗ state_cell_tgt k ov ∗
-        ((state_cell_src k ov ∗ state_cell_tgt k ov) -∗ EqR)) →
-    ⊢ isim_fsem fl_src fl_tgt (Ist ∗ EqR)%I ctx
-        (SB.sandbox_body (msk, itr)) (SB.sandbox_body (msk, itr)).
-  Proof using.
-    intros Hset Hget. rewrite /isim_fsem.
-    iIntros "!#" (arg) "[I E] _".
-    rewrite /SB.sandbox_body /=. iApply isim_refl.
-    - intros k v' Hmsk. iIntros "[I E]".
-      iPoseProof (Hset k v' Hmsk with "E") as
-        (ov) "(SRC & TGT & CLOSE)".
-      iExists ov. iFrame "SRC TGT". iIntros "[SRC TGT]".
-      iSplitL "I"; first done. iApply ("CLOSE" with "[$SRC $TGT]").
-    - intros k Hmsk. iIntros "[I E]".
-      iPoseProof (Hget k Hmsk with "E") as
-        (ov) "(SRC & TGT & CLOSE)".
-      iExists ov. iFrame "SRC TGT". iIntros "[SRC TGT]".
-      iSplitL "I"; first done. iApply ("CLOSE" with "[$SRC $TGT]").
-    - iFrame.
-  Qed.
-
-End ISIM_REFL.
-
-Local Lemma mod_add_scope_set `{Σ : GRA} (m1 m2 : Mod.t) :
-  (list_to_set (Mod.scopes (m1 ★ m2)) : gset string) =
-    list_to_set (Mod.scopes m1) ∪ list_to_set (Mod.scopes m2).
-Proof.
-  apply set_eq. intros scope.
-  rewrite elem_of_list_to_set elem_of_union /=.
-  rewrite sorting.merge_sort_Permutation elem_of_app.
-  by rewrite !elem_of_list_to_set.
-Qed.
-
-Local Lemma mod_add_scope_disjoint `{Σ : GRA} (m1 m2 : Mod.t)
-    (WF : Mod.wf (m1 ★ m2)) :
-  (list_to_set (Mod.scopes m1) : gset string) ##
-    list_to_set (Mod.scopes m2).
-Proof.
-  intros scope IN1 IN2.
-  rewrite !elem_of_list_to_set in IN1, IN2.
-  pose proof (Mod.wf_scopes _ WF) as ND.
-  rewrite /= sorting.merge_sort_Permutation NoDup_app in ND.
-  destruct ND as [_ [DISJ _]]. exact (DISJ scope IN1 IN2).
-Qed.
-
-Local Lemma state_slice_union_with_l
-    (S1 S2 : gset string) (m1 m2 : gmap key (option Any.t))
-    (SCOPED2 : set_map fst (dom m2) ⊆ S2) (DISJ : S1 ## S2) :
-  state_slice S1 (union_with uwnd m1 m2) = state_slice S1 m1.
-Proof.
-  apply map_eq. intros k. rewrite !state_slice_lookup.
-  destruct (decide (k.1 ∈ S1)) as [IN|NIN]; last done.
-  rewrite lookup_union_with.
-  destruct (m2 !! k) eqn:LOOK2; last by destruct (m1 !! k).
-  exfalso. apply elem_of_dom_2 in LOOK2.
-  apply (DISJ k.1 IN), SCOPED2.
-  apply elem_of_map. exists k. done.
-Qed.
-
-Local Lemma state_slice_union_with_r
-    (S1 S2 : gset string) (m1 m2 : gmap key (option Any.t))
-    (SCOPED1 : set_map fst (dom m1) ⊆ S1) (DISJ : S1 ## S2) :
-  state_slice S2 (union_with uwnd m1 m2) = state_slice S2 m2.
-Proof.
-  apply map_eq. intros k. rewrite !state_slice_lookup.
-  destruct (decide (k.1 ∈ S2)) as [IN|NIN]; last done.
-  rewrite lookup_union_with.
-  destruct (m1 !! k) eqn:LOOK1; last by destruct (m2 !! k).
-  exfalso. apply elem_of_dom_2 in LOOK1.
-  apply (DISJ k.1).
-  - apply SCOPED1, elem_of_map. exists k. done.
-  - exact IN.
-Qed.
-
-Section ISIM_MODULE_REFL.
+Section ISIM_MODULE_REFL_COMPOSITION.
   Context `{!crisG Γ Σ α β τ _S _I}.
 
-  Lemma ISim_refl (ctx : contextuality) (M : Mod.t) :
-    ⊢ ISim.t ctx M M (IstEq M).
-  Proof.
-    rewrite /ISim.t. iIntros (WF).
-    iSplit.
-    { iPureIntro. split; first done. destruct WF; done. }
-    iIntros (STATE0).
-    iSplit.
-    { iIntros "SRC TGT".
-      iApply (@state_eq_init_same Σ STATE0 (list_to_set (Mod.scopes M))
-        (Mod.initial_st M) with "SRC TGT"). }
-    iIntros (fn). rewrite /ISim.sim_fun.
-    iIntros "%WFS %WFT" (fs) "%Hfs".
-    rewrite lookup_fmap in Hfs.
-    destruct (Mod.fnsems M !! fn) as [[[fmsk fbdy]|]|] eqn:Hc; ss.
-    hexploit (Mod.well_scoped_fns M fn (fmsk, fbdy)).
-    { rewrite lookup_omap Hc //. }
-    intros [HPUT HGET].
-    clarify. iExists (SB.sandbox_body (fmsk, fbdy)).
-    iSplit; first by rewrite /sandbox_fnsemmap lookup_fmap Hc.
-    rewrite /isim_fsem. iIntros "!#" (arg) "IST _".
-    rewrite /SB.sandbox_body /=. iApply (@isim_refl Σ STATE0).
-    - intros k v Hmsk. iApply (@state_eq_put Σ STATE0).
-      rewrite elem_of_list_to_set. eapply HPUT. exact Hmsk.
-    - intros k Hmsk. iApply (@state_eq_get Σ STATE0).
-      rewrite elem_of_list_to_set. eapply HGET. exact Hmsk.
-    - iFrame.
-  Qed.
-
-  Lemma ISim_reflL
-      (ctx : contextuality) (A B C : Mod.t)
+  Local Lemma ISim_sim_funs_reflL_open (C : Mod.t)
       (Ist : stateGS Σ → iProp Σ) :
-    Mod.scopes A ⊆+ Mod.scopes B →
-    dom (Mod.fnsems A) ⊆ dom (Mod.fnsems B) →
-    (Mod.wf B → map_Forall (const is_Some) (Mod.fnsems A)) →
-    (∀ (STATE : stateGS Σ) fn,
-      ⌜fn ∈ dom (Mod.fnsems A)⌝ →
-      @ISim.sim_fun Γ Σ α β _S _I ctx (C ★ A) (C ★ B)
-        (λ STATE, (IstEq C STATE ∗ Ist STATE)%I) STATE fn) -∗
-    (∀ STATE,
-      state_init_src (list_to_set (Mod.scopes A))
-        (Mod.initial_st A) STATE -∗
-      state_init_tgt (list_to_set (Mod.scopes B))
-        (Mod.initial_st B) STATE -∗
-      Ist STATE) -∗
-      ISim.t ctx (C ★ A) (C ★ B)
-        (λ STATE, (IstEq C STATE ∗ Ist STATE)%I).
-  Proof using.
-    intros Hscp Hfns Hnodup.
-    iIntros "Hsim Hinit". rewrite /ISim.t. iIntros (WFT).
-    pose (SC := (list_to_set (Mod.scopes C) : gset string)).
-    pose (SA := (list_to_set (Mod.scopes A) : gset string)).
-    pose (SB := (list_to_set (Mod.scopes B) : gset string)).
-    assert (SDISJ_CB : SC ## SB).
-    { subst SC SB. apply mod_add_scope_disjoint. exact WFT. }
-    assert (SA_SUB : SA ⊆ SB).
-    { intros scope IN.
-      rewrite /SA elem_of_list_to_set in IN.
-      rewrite /SB elem_of_list_to_set.
-      eapply elem_of_submseteq; eauto. }
-    assert (SDISJ_CA : SC ## SA) by set_solver.
-    assert (SLICE_SRC_C :
-      state_slice SC (Mod.initial_st (C ★ A)) =
-        state_slice SC (Mod.initial_st C)).
-    { apply state_slice_union_with_l with (S2 := SA).
-      - apply Mod.well_scoped_init.
-      - exact SDISJ_CA. }
-    assert (SLICE_SRC_A :
-      state_slice SA (Mod.initial_st (C ★ A)) =
-        state_slice SA (Mod.initial_st A)).
-    { apply state_slice_union_with_r with (S1 := SC).
-      - apply Mod.well_scoped_init.
-      - exact SDISJ_CA. }
-    assert (SLICE_TGT_C :
-      state_slice SC (Mod.initial_st (C ★ B)) =
-        state_slice SC (Mod.initial_st C)).
-    { apply state_slice_union_with_l with (S2 := SB).
-      - apply Mod.well_scoped_init.
-      - exact SDISJ_CB. }
-    assert (SLICE_TGT_B :
-      state_slice SB (Mod.initial_st (C ★ B)) =
-        state_slice SB (Mod.initial_st B)).
-    { apply state_slice_union_with_r with (S1 := SC).
-      - apply Mod.well_scoped_init.
-      - exact SDISJ_CB. }
-    destruct (Mod.add_wf_inv C B WFT) as
-      [WFC [WFB [FNSDISJ SCOPEND]]].
-    iSplit.
-    { iPureIntro. split.
-      { rewrite /= !sorting.merge_sort_Permutation.
-        apply submseteq_app; [done | exact Hscp]. }
-      eapply map_Forall_union_with.
-      { set_solver. }
-      split; [apply WFC | apply Hnodup, WFB].
-    }
-    iIntros (STATE). iSplitL "Hinit".
-    { iIntros "SRC TGT".
-      iEval (rewrite (mod_add_scope_set C A)) in "SRC".
-      iEval (rewrite (mod_add_scope_set C B)) in "TGT".
-      iPoseProof (state_init_src_union SC SA
-        (Mod.initial_st (C ★ A)) SDISJ_CA with "SRC") as
-        "[SRCC SRCA]".
-      iPoseProof (state_init_tgt_union SC SB
-        (Mod.initial_st (C ★ B)) SDISJ_CB with "TGT") as
-        "[TGTC TGTB]".
-      iPoseProof (state_init_src_ext SC (Mod.initial_st (C ★ A))
-        (Mod.initial_st C) SLICE_SRC_C with "SRCC") as "SRCC".
-      iPoseProof (state_init_src_ext SA (Mod.initial_st (C ★ A))
-        (Mod.initial_st A) SLICE_SRC_A with "SRCA") as "SRCA".
-      iPoseProof (state_init_tgt_ext SC (Mod.initial_st (C ★ B))
-        (Mod.initial_st C) SLICE_TGT_C with "TGTC") as "TGTC".
-      iPoseProof (state_init_tgt_ext SB (Mod.initial_st (C ★ B))
-        (Mod.initial_st B) SLICE_TGT_B with "TGTB") as "TGTB".
-      iSplitL "SRCC TGTC".
-      - rewrite /IstEq.
-        iApply (state_eq_init_same with "SRCC TGTC").
-      - iApply ("Hinit" $! STATE with "SRCA TGTB"). }
-    iIntros (fn).
-    destruct (decide (fn ∈ dom (Mod.fnsems A))) as [Hin|Hnin].
-    { iApply ("Hsim" $! STATE fn). done. }
-    apply not_elem_of_dom in Hnin.
-    rewrite /ISim.sim_fun.
-    iIntros "%WFS %WFT2" (fs) "%Hsrc".
-    rewrite lookup_fmap lookup_union_with Hnin in Hsrc.
+    ⊢ ISim.sim_funs open C C
+        (λ STATE, (IstEq C STATE ∗ Ist STATE)%I) C C.
+  Proof.
+    rewrite /ISim.sim_funs. iIntros (WFC). iSplit.
+    { iPureIntro. split; [apply WFC | done]. }
+    iIntros (fn) "%Hfn". rewrite /ISim.sim_fun.
+    iIntros (STATE).
+    iIntros "%WFS %WFT" (fs) "%Hsrc".
+    rewrite lookup_fmap in Hsrc.
     destruct (Mod.fnsems C !! fn)
-      as [[[fmsksrc fbdysrc]|]|] eqn:Hc; ss.
-    clarify.
-    destruct (Mod.fnsems B !! fn) as [fnt|] eqn:Hb.
-    { exfalso. inv WFT2.
-      rewrite map_Forall_lookup in wf_fns.
-      hexploit (wf_fns fn).
-      { rewrite lookup_union_with Hc Hb //=. }
-      intros []; done.
-    }
-    hexploit (Mod.well_scoped_fns C fn (fmsksrc, fbdysrc)).
+      as [[[fmsk fbdy]|]|] eqn:Hc; ss.
+    hexploit (Mod.well_scoped_fns C fn (fmsk, fbdy)).
     { rewrite lookup_omap Hc //. }
-    intros [HPUT HGET].
-    iExists (SB.sandbox_body (fmsksrc, fbdysrc)).
-    iSplit.
-    { iPureIntro.
-      rewrite /sandbox_fnsemmap lookup_fmap lookup_union_with Hc Hb //. }
+    intros [HPUT HGET]. clarify.
+    iExists (SB.sandbox_body (fmsk, fbdy)).
+    iSplit; first by rewrite /sandbox_fnsemmap lookup_fmap Hc.
     iApply (@isim_reflL Γ Σ α β _S _I STATE).
     - intros k v Hmsk. iApply (@state_eq_put Σ STATE).
       rewrite /IstEq elem_of_list_to_set. eapply HPUT. exact Hmsk.
@@ -470,286 +33,92 @@ Section ISIM_MODULE_REFL.
       rewrite /IstEq elem_of_list_to_set. eapply HGET. exact Hmsk.
   Qed.
 
+  Lemma ISim_sim_funs_reflL
+      (ctx : contextuality) (A B C : Mod.t)
+      (Ist : stateGS Σ → iProp Σ) :
+    ⊢ ISim.sim_funs ctx (C ★ A) (C ★ B)
+        (λ STATE, (IstEq C STATE ∗ Ist STATE)%I) C C.
+  Proof.
+    iApply (ISim_sim_funs_extend_ctx ctx C C A B
+      (λ STATE, (IstEq C STATE ∗ Ist STATE)%I) C C).
+    - done.
+    - iApply ISim_sim_funs_reflL_open.
+  Qed.
+
+  Lemma ISim_sim_funs_reflR
+      (ctx : contextuality) (A B C : Mod.t)
+      (Ist : stateGS Σ → iProp Σ) :
+    ⊢ ISim.sim_funs ctx (A ★ C) (B ★ C)
+        (λ STATE, (Ist STATE ∗ IstEq C STATE)%I) C C.
+  Proof.
+    rewrite (comm _ A C) (comm _ B C).
+    iApply (ISim_sim_funs_frame ctx (C ★ A) (C ★ B)
+      (IstEq C) Ist C C).
+    iApply (ISim_sim_funs_extend_ctx ctx C C A B (IstEq C) C C).
+    - done.
+    - iApply (ISim_sim_funs_refl open C).
+  Qed.
+
+  Lemma ISim_reflL
+      (ctx : contextuality) (A B C : Mod.t)
+      (Ist : stateGS Σ → iProp Σ) :
+    ISim.init_ist A B Ist -∗
+    ISim.sim_funs ctx (C ★ A) (C ★ B)
+      (λ STATE, (IstEq C STATE ∗ Ist STATE)%I) A B -∗
+    ISim.t ctx (C ★ A) (C ★ B)
+      (λ STATE, (IstEq C STATE ∗ Ist STATE)%I).
+  Proof.
+    iIntros "INIT SIM". rewrite /ISim.t. iSplit.
+    - iApply add_init_ist. iSplitR "INIT".
+      + iApply ISim_init_ist_refl.
+      + done.
+    - iApply add_sim_funs. iSplitR "SIM".
+      + iApply ISim_sim_funs_reflL.
+      + done.
+  Qed.
+
   Lemma ISim_reflR
       (ctx : contextuality) (A B C : Mod.t)
       (Ist : stateGS Σ → iProp Σ) :
-    Mod.scopes A ⊆+ Mod.scopes B →
-    dom (Mod.fnsems A) ⊆ dom (Mod.fnsems B) →
-    (Mod.wf B → map_Forall (const is_Some) (Mod.fnsems A)) →
-    (∀ (STATE : stateGS Σ) fn,
-      ⌜fn ∈ dom (Mod.fnsems A)⌝ →
-      @ISim.sim_fun Γ Σ α β _S _I ctx (A ★ C) (B ★ C)
-        (λ STATE, (Ist STATE ∗ IstEq C STATE)%I) STATE fn) -∗
-    (∀ STATE,
-      state_init_src (list_to_set (Mod.scopes A))
-        (Mod.initial_st A) STATE -∗
-      state_init_tgt (list_to_set (Mod.scopes B))
-        (Mod.initial_st B) STATE -∗
-      Ist STATE) -∗
-      ISim.t ctx (A ★ C) (B ★ C)
-        (λ STATE, (Ist STATE ∗ IstEq C STATE)%I).
-  Proof using.
-    intros Hscp Hfns Hnodup.
-    iIntros "Hsim Hinit". rewrite /ISim.t. iIntros (WFT).
-    pose (SA := (list_to_set (Mod.scopes A) : gset string)).
-    pose (SB := (list_to_set (Mod.scopes B) : gset string)).
-    pose (SC := (list_to_set (Mod.scopes C) : gset string)).
-    assert (SDISJ_BC : SB ## SC).
-    { subst SB SC. apply mod_add_scope_disjoint. exact WFT. }
-    assert (SA_SUB : SA ⊆ SB).
-    { intros scope IN.
-      rewrite /SA elem_of_list_to_set in IN.
-      rewrite /SB elem_of_list_to_set.
-      eapply elem_of_submseteq; eauto. }
-    assert (SDISJ_AC : SA ## SC) by set_solver.
-    assert (SLICE_SRC_A :
-      state_slice SA (Mod.initial_st (A ★ C)) =
-        state_slice SA (Mod.initial_st A)).
-    { apply state_slice_union_with_l with (S2 := SC).
-      - apply Mod.well_scoped_init.
-      - exact SDISJ_AC. }
-    assert (SLICE_SRC_C :
-      state_slice SC (Mod.initial_st (A ★ C)) =
-        state_slice SC (Mod.initial_st C)).
-    { apply state_slice_union_with_r with (S1 := SA).
-      - apply Mod.well_scoped_init.
-      - exact SDISJ_AC. }
-    assert (SLICE_TGT_B :
-      state_slice SB (Mod.initial_st (B ★ C)) =
-        state_slice SB (Mod.initial_st B)).
-    { apply state_slice_union_with_l with (S2 := SC).
-      - apply Mod.well_scoped_init.
-      - exact SDISJ_BC. }
-    assert (SLICE_TGT_C :
-      state_slice SC (Mod.initial_st (B ★ C)) =
-        state_slice SC (Mod.initial_st C)).
-    { apply state_slice_union_with_r with (S1 := SB).
-      - apply Mod.well_scoped_init.
-      - exact SDISJ_BC. }
-    destruct (Mod.add_wf_inv B C WFT) as
-      [WFB [WFC [FNSDISJ SCOPEND]]].
-    iSplit.
-    { iPureIntro. split.
-      { rewrite /= !sorting.merge_sort_Permutation.
-        apply submseteq_app; [exact Hscp | done]. }
-      eapply map_Forall_union_with.
-      { set_solver. }
-      split; [apply Hnodup, WFB | apply WFC].
-    }
-    iIntros (STATE). iSplitL "Hinit".
-    { iIntros "SRC TGT".
-      iEval (rewrite (mod_add_scope_set A C)) in "SRC".
-      iEval (rewrite (mod_add_scope_set B C)) in "TGT".
-      iPoseProof (state_init_src_union SA SC
-        (Mod.initial_st (A ★ C)) SDISJ_AC with "SRC") as
-        "[SRCA SRCC]".
-      iPoseProof (state_init_tgt_union SB SC
-        (Mod.initial_st (B ★ C)) SDISJ_BC with "TGT") as
-        "[TGTB TGTC]".
-      iPoseProof (state_init_src_ext SA (Mod.initial_st (A ★ C))
-        (Mod.initial_st A) SLICE_SRC_A with "SRCA") as "SRCA".
-      iPoseProof (state_init_src_ext SC (Mod.initial_st (A ★ C))
-        (Mod.initial_st C) SLICE_SRC_C with "SRCC") as "SRCC".
-      iPoseProof (state_init_tgt_ext SB (Mod.initial_st (B ★ C))
-        (Mod.initial_st B) SLICE_TGT_B with "TGTB") as "TGTB".
-      iPoseProof (state_init_tgt_ext SC (Mod.initial_st (B ★ C))
-        (Mod.initial_st C) SLICE_TGT_C with "TGTC") as "TGTC".
-      iSplitR "SRCC TGTC".
-      - iApply ("Hinit" $! STATE with "SRCA TGTB").
-      - rewrite /IstEq.
-        iApply (state_eq_init_same with "SRCC TGTC"). }
-    iIntros (fn).
-    destruct (decide (fn ∈ dom (Mod.fnsems A))) as [Hin|Hnin].
-    { iApply ("Hsim" $! STATE fn). done. }
-    apply not_elem_of_dom in Hnin.
-    rewrite /ISim.sim_fun.
-    iIntros "%WFS %WFT2" (fs) "%Hsrc".
-    rewrite lookup_fmap lookup_union_with Hnin in Hsrc.
-    destruct (Mod.fnsems C !! fn)
-      as [[[fmsksrc fbdysrc]|]|] eqn:Hc; ss.
-    clarify.
-    destruct (Mod.fnsems B !! fn) as [fnt|] eqn:Hb.
-    { exfalso. inv WFT2.
-      rewrite map_Forall_lookup in wf_fns.
-      hexploit (wf_fns fn).
-      { rewrite lookup_union_with Hc Hb //=. }
-      intros []; done.
-    }
-    hexploit (Mod.well_scoped_fns C fn (fmsksrc, fbdysrc)).
-    { rewrite lookup_omap Hc //. }
-    intros [HPUT HGET].
-    iExists (SB.sandbox_body (fmsksrc, fbdysrc)).
-    iSplit.
-    { iPureIntro.
-      rewrite /sandbox_fnsemmap lookup_fmap lookup_union_with Hc Hb //. }
-    iApply (@isim_reflR Γ Σ α β _S _I STATE).
-    - intros k v Hmsk. iApply (@state_eq_put Σ STATE).
-      rewrite /IstEq elem_of_list_to_set. eapply HPUT. exact Hmsk.
-    - intros k Hmsk. iApply (@state_eq_get Σ STATE).
-      rewrite /IstEq elem_of_list_to_set. eapply HGET. exact Hmsk.
+    ISim.init_ist A B Ist -∗
+    ISim.sim_funs ctx (A ★ C) (B ★ C)
+      (λ STATE, (Ist STATE ∗ IstEq C STATE)%I) A B -∗
+    ISim.t ctx (A ★ C) (B ★ C)
+      (λ STATE, (Ist STATE ∗ IstEq C STATE)%I).
+  Proof.
+    iIntros "INIT SIM". rewrite /ISim.t. iSplit.
+    - iApply add_init_ist. iSplitL "INIT".
+      + done.
+      + iApply ISim_init_ist_refl.
+    - iApply add_sim_funs. iSplitL "SIM".
+      + done.
+      + iApply ISim_sim_funs_reflR.
   Qed.
 
-End ISIM_MODULE_REFL.
+End ISIM_MODULE_REFL_COMPOSITION.
 
-Section STATE_EQ_RULES.
-
+Section ISIM_CONTEXT_EXTENSION.
   Context `{!crisG Γ Σ α β τ _S _I}.
-  Context `{STATE : !stateGS Σ}.
 
-  #[local] Set Implicit Arguments.
-
-  Lemma isim_sput_eq ctx fl_s fl_t S g {Rs Rt} RR ps pt k v' k_s k_t
-      (IN : k.1 ∈ S) :
-    state_eq S STATE ∗
-      (state_eq S STATE -∗
-        @isim Σ _ ctx fl_s fl_t (state_eq S STATE) g Rs Rt RR
-          true true (k_s tt) (k_t tt)) ⊢
-    @isim Σ _ ctx fl_s fl_t (state_eq S STATE) g Rs Rt RR ps pt
-      (trigger (SPut k v') >>= k_s) (trigger (SPut k v') >>= k_t).
+  Lemma ISim_ctx (ms mt C : Mod.t) Ist :
+    ISim.t open ms mt Ist ⊢
+    ISim.t open (ms ★ C) (mt ★ C)
+      (λ STATE, (IstEq C STATE ∗ Ist STATE)%I).
   Proof.
-    iIntros "[EQ SIM]".
-    iPoseProof (state_eq_put S k v' IN with "EQ") as
-      (ov) "(SRC & TGT & CLOSE)".
-    destruct ov as [v|].
-    - iEval (rewrite /state_cell_src /state_cell_tgt /=) in "SRC TGT".
-      iApply isim_sput_src. iFrame "SRC". iIntros "SRC".
-      iApply isim_sput_tgt. iFrame "TGT". iIntros "TGT".
-      iApply "SIM". iApply ("CLOSE" with "[$SRC $TGT]").
-    - iEval (rewrite /state_cell_src /state_cell_tgt /=) in "SRC TGT".
-      iApply isim_sput_src_uninit. iFrame "SRC". iIntros "SRC".
-      iApply isim_sput_tgt_uninit. iFrame "TGT". iIntros "TGT".
-      iApply "SIM". iApply ("CLOSE" with "[$SRC $TGT]").
+    rewrite -(comm _ C ms) -(comm _ C mt).
+    rewrite /ISim.t. iIntros "[INIT FUNS]".
+    iSplitL "INIT".
+    - iApply add_init_ist. iSplitR "INIT".
+      + iApply ISim_init_ist_refl.
+      + done.
+    - iApply add_sim_funs. iSplitR "FUNS".
+      + iApply ISim_sim_funs_reflL.
+      + rewrite (comm _ C ms) (comm _ C mt).
+        iApply (ISim_sim_funs_frame open (ms ★ C) (mt ★ C)
+          Ist (IstEq C) ms mt).
+        iApply (ISim_sim_funs_extend_ctx open ms mt C C Ist ms mt).
+        * done.
+        * done.
   Qed.
 
-  Lemma isim_sget_eq ctx fl_s fl_t S g {Rs Rt} RR ps pt k k_s k_t
-      (IN : k.1 ∈ S) :
-    state_eq S STATE ∗
-      (∀ v, state_eq S STATE -∗
-        @isim Σ _ ctx fl_s fl_t (state_eq S STATE) g Rs Rt RR
-          true true (k_s v) (k_t v)) ⊢
-    @isim Σ _ ctx fl_s fl_t (state_eq S STATE) g Rs Rt RR ps pt
-      (trigger (SGet k) >>= k_s) (trigger (SGet k) >>= k_t).
-  Proof.
-    iIntros "[EQ SIM]".
-    iPoseProof (state_eq_get S k IN with "EQ") as
-      (ov) "(SRC & TGT & CLOSE)".
-    destruct ov as [v|].
-    - iEval (rewrite /state_cell_src /state_cell_tgt /=) in "SRC TGT".
-      iApply isim_sget_src. iFrame "SRC". iIntros "SRC".
-      iApply isim_sget_tgt. iFrame "TGT". iIntros "TGT".
-      iApply ("SIM" $! v). iApply ("CLOSE" with "[$SRC $TGT]").
-    - iEval (rewrite /state_cell_src /state_cell_tgt /=) in "SRC TGT".
-      iApply isim_sget_src_uninit. iFrame "SRC". iIntros "SRC".
-      iApply isim_sget_tgt_uninit. iFrame "TGT". iIntros "TGT".
-      iApply ("SIM" $! (tt↑)). iApply ("CLOSE" with "[$SRC $TGT]").
-  Qed.
-
-End STATE_EQ_RULES.
-
-(* Section LAT.
-  Context `{_crisG: !crisG Γ Σ α β τ _S _I}.
-
-  Lemma isim_lat_real_to_img
-      peeking img fsp lbody_s lbody_t body_s body_t fl_s fl_t msk scp ps pt st arg
-      (EQITL: eqit eq false true
-              (SB.sandbox true msk scp (SModTr.trans img sp_none lbody_s))
-              (SB.sandbox false msk scp (SModTr.trans img sp_none lbody_t)))
-      (EQIT: eqit eq false true
-              (SB.sandbox true msk scp (SModTr.trans img sp_none (body_s arg)))
-              (SB.sandbox false msk scp (SModTr.trans img sp_none (body_t arg))))
-    :
-    ⊢
-    isim open fl_s fl_t IstEq ibot ibot (ist_with_eq IstEq) ps pt
-      (st, SB.sandbox true msk scp (SModTr.trans img sp_none (lat_img peeking fsp lbody_s body_s arg)))
-      (st, SB.sandbox false msk scp (SModTr.trans img sp_none (lat_real peeking fsp lbody_t body_t arg))).
-  Proof using.
-    destruct fsp as [m pre post].
-    iApply isim_reset. clear ps pt. iStopProof. revert st.
-    eapply isim_coind. intros g Hg CIH st. iIntros. destruct_quant CIH.
-    rewrite /lat_img /lat_real.
-    unfoldIterS. unfoldIterT. rewrite {1}/lat_img_body {1}/lat_real_body.
-    cNormS. cNormT. iApply isim_bind. iSplitL "".
-    { iApply isim_eqit_tgt; et.
-      iApply isim_refl; et; i; iIntros "%"; subst; et.
-    }
-    iIntros (????) "%"; des; subst.
-    isteps_s. isteps_t.
-    destruct (peeking); cycle 1.
-    {
-      isteps_s. isteps_t.
-      iApply isim_bind. iSplitL "".
-      { iApply isim_eqit_tgt; et.
-        iApply isim_refl; et; i; iIntros "%"; subst; et.
-      }
-
-      iIntros (????) "%"; des; subst.
-      isteps_s. isteps_t.
-      iforce_t. iFrame. iIntros "GRT".
-      iforce_s. iFrame. isteps_s. isteps_t.
-      istep; et.
-    }
-
-    isteps_t. destruct _q0.
-    { iforce_t. iFrame. iIntros "GRT".
-      iforce_s true. isteps_s. iforce_s. iFrame. isteps_s. isteps_t.
-      iby_coind CIH; et.
-    }
-
-    iforce_s false. isteps_s. isteps_t.
-    iApply isim_bind. iSplitL "".
-    { iApply isim_eqit_tgt; et.
-      iApply isim_refl; et; i; iIntros "%"; subst; et.
-    }
-
-    iIntros (????) "%"; des; subst.
-    isteps_s. isteps_t.
-    iforce_t. iFrame. iIntros "GRT".
-    iforce_s. iFrame. isteps_s. isteps_t.
-    istep; et.
-  Qed.
-
-  Lemma isim_lat_img_to_hoare fsp img body_s body_t fl_s fl_t msk scp ps pt st arg
-    (EQIT: eqit eq false true
-            (SB.sandbox true msk scp (body_s arg))
-            (SB.sandbox true msk scp (SModTr.trans img sp_none (body_t arg))))
-    :
-    ⊢
-    isim open fl_s fl_t IstEq ibot ibot (ist_with_eq IstEq) ps pt
-      (st, SB.sandbox true msk scp (SModTr.HoareFun (Some (to_fspec fsp)) body_s arg))
-      (st, SB.sandbox true msk scp (SModTr.trans img sp_none (lat_img false fsp (Ret ()) body_t arg))).
-  Proof using.
-    iIntros. isteps_s. rewrite /lat_img /lat_img_body. unfoldIterT. isteps_t.
-    destruct fsp. destruct PHY as [P1 P2]. iPoseProof (P1 with "ASM") as "->".
-    iforces_r. iFrame. isteps_t.
-    iApply isim_bind. iSplitL "".
-    { iApply isim_eqit_tgt; et.
-      iApply isim_refl; et; i; iIntros "%"; subst; et.
-    }
-    iIntros (?????). des; subst.
-    isteps_t. iforces_l. iFrame.
-    istep. et.
-  Qed.
-
-  Lemma isim_lat_real_to_hoare fsp img body_s body_t fl_s fl_t msk scp ps pt st arg
-    (EQIT: eqit eq false true
-            (SB.sandbox true msk scp (body_s arg))
-            (SB.sandbox false msk scp (SModTr.trans img sp_none (body_t arg))))
-    :
-    ⊢
-    isim open fl_s fl_t IstEq ibot ibot (ist_with_eq IstEq) ps pt
-      (st, SB.sandbox true msk scp (SModTr.HoareFun (Some (to_fspec fsp)) body_s arg))
-      (st, SB.sandbox false msk scp (SModTr.trans img sp_none (lat_real false fsp (Ret ()) body_t arg))).
-  Proof using.
-    iIntros. isteps_s. rewrite /lat_real /lat_real_body. unfoldIterT. isteps_t.
-    destruct fsp. destruct PHY as [P1 P2]. iPoseProof (P1 with "ASM") as "->".
-    iApply isim_bind. iSplitL "".
-    { iApply isim_eqit_tgt; et.
-      iApply isim_refl; et; i; iIntros "%"; subst; et.
-    }
-    iIntros (????) "%"; des; subst.
-    isteps_s. isteps_t.
-    iforce_t. iFrame. iIntros "GRT".
-    iforces_l. iFrame.
-    isteps_s. isteps_t. istep; et.
-  Qed.
-End LAT. *)
+End ISIM_CONTEXT_EXTENSION.
