theories/cancellation/MInlineElim.v
@@ -26,19 +26,23 @@ Proof using _I _S crisG0 Γ Σ α β τ.
       (IstEq md STATE) closed
       (SB.sandbox_body f) (SB.sandbox_body (inline_fsem md f))).
   { intros FSIMS.
-    rewrite /ISim.t.
-    iIntros (WF). iSplit.
-    { iPureIntro. split; first done.
-      destruct WF as [wf_fns wf_scopes].
-      intros fn value Hlookup. destruct value; first ss.
-      exfalso. exploit (wf_fns fn None); [|intros []; ss].
-      rewrite /= lookup_fmap Hlookup //. }
-    iIntros (STATE). iSplit.
-    { iIntros "SRC TGT".
+    rewrite /ISim.t. iSplit.
+    { rewrite /ISim.init_ist. iIntros (WF). iSplit.
+      { done. }
+      iIntros (STATE) "SRC TGT".
       iApply (@state_eq_init_same Σ STATE
         (list_to_set (Mod.scopes md)) (Mod.initial_st md) with "SRC TGT"). }
+    rewrite /ISim.sim_funs. iIntros (WF). iSplit.
+    { iPureIntro.
+      split.
+      - destruct WF as [wf_fns wf_scopes].
+        intros fn value Hlookup. destruct value; first ss.
+        exfalso. exploit (wf_fns fn None); [|intros []; ss].
+        rewrite /= lookup_fmap Hlookup //.
+      - rewrite /MInline.inline /Mod.fnsems /= dom_fmap. done. }
+    iIntros (fn) "%Hfn". rewrite /ISim.sim_fun.
+    iIntros (STATE).
     iPoseProof (FSIMS STATE) as "#FSIMS".
-    iIntros (fn). rewrite /ISim.sim_fun.
     iIntros "%WFS %WFT" (fs) "%Hfs".
     rewrite /sandbox_fnsemmap lookup_fmap in Hfs.
     destruct (Mod.fnsems md !! fn) as [[[msk body]|]|]
