theories/filter/CallFilter.v
@@ -99,14 +99,21 @@ Module CFilter. Section CFilter.
   Lemma sim_filter_intro (bl : gset string) (m : Mod.t) :
     ⊢ ISim.t open (filter bl m) m (IstEq m).
   Proof using.
-    cStartModSim; et.
-    { ii. rr. destruct x; et.
-      exfalso. rewrite lookup_fmap in H. destruct (_ !! _) eqn: mi; ss.
-      eapply Hwf in mi. rr in mi. des; subst. ss.
-    }
-    iApply (state_eq_init_same with "SRC TGT").
+    rewrite /ISim.t. iSplit.
+    { rewrite /ISim.init_ist. iIntros (Hwf). iSplit.
+      { done. }
+      iIntros (STATE) "SRC TGT".
+      iApply (state_eq_init_same with "SRC TGT"). }
+    rewrite /ISim.sim_funs. iIntros (Hwf). iSplit.
+    { iPureIntro. split.
+      - ii. rr. destruct x; et.
+        exfalso. rewrite lookup_fmap in H. destruct (_ !! _) eqn: mi; ss.
+        eapply Hwf in mi. rr in mi. des; subst. ss.
+      - rewrite /filter /Mod.fnsems /= dom_fmap. done. }
+    iIntros (fn) "%Hfn".
 
     rewrite /ISim.sim_fun ?lookup_fmap.
+    iIntros (STATE).
     iIntros "%WFS %WFT" (fs) "%Hfs".
     destruct (_ !! _) as [[[msk bd]|]|] eqn : Ht; ss.
     hexploit (Mod.well_scoped_fns m fn (msk, bd)).
@@ -172,23 +179,26 @@ Module CFilter. Section CFilter.
       (SUB : get_fids (dom (m.(Mod.fnsems))) ## bl) :
     ⊢ ISim.t closed m (filter bl m) (IstEq m).
   Proof using.
-    rewrite /ISim.t. iIntros (Hwf).
-    iSplit.
-    { iPureIntro. split; first done.
-      destruct Hwf as [wf_fns _].
-      rewrite map_Forall_lookup in wf_fns |- *.
-      intros i x Hix. specialize (wf_fns i).
-      rewrite /filter /Mod.fnsems /= lookup_fmap Hix /= in wf_fns.
-      destruct x as [[msk bd]|]; ss.
-      eapply wf_fns. reflexivity.
-    }
-    iIntros (STATE). iSplit.
-    { iIntros "SRC TGT".
+    rewrite /ISim.t. iSplit.
+    { rewrite /ISim.init_ist. iIntros (Hwf). iSplit.
+      { done. }
+      iIntros (STATE) "SRC TGT".
       iApply (@state_eq_init_same Σ STATE
         (list_to_set (Mod.scopes m)) (Mod.initial_st m) with "SRC TGT"). }
-    iIntros (fn).
+    rewrite /ISim.sim_funs. iIntros (Hwf). iSplit.
+    { iPureIntro.
+      split.
+      - destruct Hwf as [wf_fns _].
+        rewrite map_Forall_lookup in wf_fns |- *.
+        intros i x Hix. specialize (wf_fns i).
+        rewrite /filter /Mod.fnsems /= lookup_fmap Hix /= in wf_fns.
+        destruct x as [[msk bd]|]; ss.
+        eapply wf_fns. reflexivity.
+      - rewrite /filter /Mod.fnsems /= dom_fmap. done. }
+    iIntros (fn) "%Hfn".
 
     rewrite /ISim.sim_fun ?lookup_fmap.
+    iIntros (STATE).
     iIntros "%WFS %WFT" (fs) "%Hfs".
     destruct (_ !! _) as [[[msk bd]|]|] eqn : Ht; ss.
     hexploit (Mod.well_scoped_fns m fn (msk, bd)).
