theories/simulations/msim/ISimExtendCtx.v
@@ -1,0 +1,156 @@
+From CRIS.common Require Import Common ConcRA StatePredicate.
+From CRIS.modules Require Import Mod.
+From CRIS.simulations.msim Require Import MSim MSimCommon ISim.
+From iris.proofmode Require Import proofmode.
+
+Local Ltac mstep_extend :=
+  guclo msimC_spec; econs; econs; eauto; econs; eauto.
+
+Local Lemma msim_extend_ctx
+    `{Σ : GRA} `{!stateGS Σ} (contextual : contextuality)
+    (Ks Kt Cs Ct : Mod.t) (Ist : iProp Σ) {Rs Rt}
+    (RR : retr_type Σ Rs Rt) ps pt
+    (itr_src : itree crisE Rs) (itr_tgt : itree crisE Rt) (fmr : Σ) :
+  Mod.wf (Ks ★ Cs) →
+  Mod.wf (Kt ★ Ct) →
+  msim open
+    (sandbox_fnsemmap (Mod.fnsems Ks))
+    (sandbox_fnsemmap (Mod.fnsems Kt))
+    Ist RR ps pt itr_src itr_tgt fmr →
+  @msim _ _ contextual
+    (sandbox_fnsemmap (Mod.fnsems (Ks ★ Cs)))
+    (sandbox_fnsemmap (Mod.fnsems (Kt ★ Ct)))
+    Ist Rs Rt RR ps pt itr_src itr_tgt fmr.
+Proof.
+  ginit.
+  intros WFS WFT.
+  move WFS at top. move WFT at top.
+  revert_until RR. gcofix CIH.
+  intros ps pt itr_src itr_tgt fmr SIM.
+  move SIM before CIH. revert_until SIM. punfold SIM.
+  pattern ps, pt, itr_src, itr_tgt, fmr.
+  eapply _msim_tarski, SIM; clear SIM fmr.
+  intros ps0 pt0 itr_src0 itr_tgt0 fmr IN.
+  guclo msim_wfC_spec. econs. intros VALID.
+  guclo msim_nodupC_spec. econs. intros NODUPS NODUPT.
+  hexploit IN; ss.
+  { move: NODUPS. rewrite ?map_Forall_lookup => H i x.
+    move: H => /(_ i x) /=.
+    rewrite ?lookup_fmap lookup_union_with.
+    destruct (_ Ks !! i) as [[[? ?]|]|];
+      destruct (_ Cs !! i); ss; intros; clarify. }
+  { move: NODUPT. rewrite ?map_Forall_lookup => H i x.
+    move: H => /(_ i x) /=.
+    rewrite ?lookup_fmap lookup_union_with.
+    destruct (_ Kt !! i) as [[[? ?]|]|];
+      destruct (_ Ct !! i); ss; intros; clarify. }
+  clear IN. intros IN.
+  destruct IN as [fmr1 [STEP UPD]]; eauto.
+  inv STEP; try by (mstep_extend; eauto).
+  - mstep_extend.
+    revert FUN.
+    intros [[f2|] [? FUN]]%lookup_fmap_Some; ss; clarify.
+    move: FUN => /(Mod.lookup_add_l).
+    move /(_ Cs WFS) => /=. rewrite lookup_fmap => -> //=.
+  - mstep_extend.
+    revert FUN.
+    intros [[f2|] [? FUN]]%lookup_fmap_Some; ss; clarify.
+    move: FUN => /(Mod.lookup_add_l).
+    move /(_ Ct WFT) => /=. rewrite lookup_fmap => -> //=.
+  - gstep. econs. econs. econs; eauto. econs; eauto.
+    gbase. pclearbot. eapply CIH; eauto.
+Qed.
+
+Local Lemma isim_extend_ctx
+    `{Σ : GRA} `{!stateGS Σ} (contextual : contextuality)
+    (Ks Kt Cs Ct : Mod.t) (Ist : iProp Σ) {Rs Rt}
+    (RR : retr_type Σ Rs Rt) ps pt
+    (itr_src : itree crisE Rs) (itr_tgt : itree crisE Rt) :
+  Mod.wf (Ks ★ Cs) →
+  Mod.wf (Kt ★ Ct) →
+  isim open
+    (sandbox_fnsemmap (Mod.fnsems Ks))
+    (sandbox_fnsemmap (Mod.fnsems Kt))
+    Ist ibot RR ps pt itr_src itr_tgt ⊢
+  @isim _ _ contextual
+    (sandbox_fnsemmap (Mod.fnsems (Ks ★ Cs)))
+    (sandbox_fnsemmap (Mod.fnsems (Kt ★ Ct)))
+    Ist ibot Rs Rt RR ps pt itr_src itr_tgt.
+Proof.
+  intros WFS WFT.
+  apply entails_pointwise => r _ SIM.
+  eapply isim_init in SIM; eauto.
+  eapply gpaco8_mon in SIM; try apply iunlift_ibot; eauto.
+  eapply gpaco8_init in SIM; eauto with paco.
+  eapply isim_final, gpaco8_final; eauto with paco. right.
+  assert (SIM' :
+    @msim _ _ contextual
+      (sandbox_fnsemmap (Mod.fnsems (Ks ★ Cs)))
+      (sandbox_fnsemmap (Mod.fnsems (Kt ★ Ct))) Ist
+      Rs Rt RR ps pt itr_src itr_tgt r).
+  { eapply msim_extend_ctx; eauto. }
+  eapply paco8_mon_bot.
+  - exact SIM'.
+  - intros; assumption.
+Qed.
+
+Local Lemma isim_fsem_extend_ctx
+    `{!crisG Γ Σ α β τ _S _I} `{!stateGS Σ}
+    (contextual : contextuality) (Ks Kt Cs Ct : Mod.t)
+    (Ist : iProp Σ) fs ft :
+  Mod.wf (Ks ★ Cs) →
+  Mod.wf (Kt ★ Ct) →
+  isim_fsem
+    (sandbox_fnsemmap (Mod.fnsems Ks))
+    (sandbox_fnsemmap (Mod.fnsems Kt)) Ist open fs ft ⊢
+  isim_fsem
+    (sandbox_fnsemmap (Mod.fnsems (Ks ★ Cs)))
+    (sandbox_fnsemmap (Mod.fnsems (Kt ★ Ct))) Ist contextual fs ft.
+Proof.
+  intros WFS WFT. rewrite /isim_fsem.
+  iIntros "#SIM !#" (arg) "IST WINV".
+  iApply (isim_extend_ctx contextual Ks Kt Cs Ct); eauto.
+  iApply ("SIM" $! arg with "IST WINV").
+Qed.
+
+Section ISIM_EXTEND_CTX.
+  Context `{!crisG Γ Σ α β τ _S _I}.
+
+  (** Transport open function simulations to larger ambient modules.  [DOM]
+      ensures that extension does not introduce a new selected source
+      function whose previous [sim_fun] obligation was vacuous. *)
+  Lemma ISim_sim_funs_extend_ctx
+      (contextual : contextuality) (Ks Kt Cs Ct : Mod.t)
+      (Ist : stateGS Σ → iProp Σ) (Ms Mt : Mod.t)
+      (DOM : dom (Mod.fnsems Ms) ⊆ dom (Mod.fnsems Ks)) :
+    ISim.sim_funs open Ks Kt Ist Ms Mt ⊢
+    ISim.sim_funs contextual (Ks ★ Cs) (Kt ★ Ct) Ist Ms Mt.
+  Proof.
+    rewrite /ISim.sim_funs. iIntros "SIM %WFMT".
+    iDestruct ("SIM" $! WFMT) as "[%PURE SIM]".
+    iSplit; first done.
+    iIntros (fn) "%IN".
+    iPoseProof ("SIM" $! fn with "[]") as "SIM"; first done.
+    rewrite /ISim.sim_fun.
+    iIntros (STATE).
+    iIntros "%WFS %WFT" (fs) "%LOOK".
+    destruct (Mod.add_wf_inv Ks Cs WFS) as [WFKS _].
+    destruct (Mod.add_wf_inv Kt Ct WFT) as [WFKT _].
+    iEval (rewrite /ISim.sim_fun) in "SIM".
+    iSpecialize ("SIM" $! STATE with "[] []"); [done|done|].
+    iSpecialize ("SIM" $! fs with "[]").
+    { iPureIntro.
+      rewrite /sandbox_fnsemmap !lookup_fmap in LOOK |- *.
+      rewrite (lookup_fnsems_l_2 Ks Cs fn WFS (DOM fn IN)) in LOOK.
+      exact LOOK. }
+    iDestruct "SIM" as (ft) "[%LOOKT FSIM]".
+    iExists ft. iSplit.
+    { iPureIntro.
+      rewrite /sandbox_fnsemmap !lookup_fmap in LOOKT |- *.
+      destruct (Mod.fnsems Kt !! fn)
+        as [[[msk body]|]|] eqn:HKT; ss; clarify.
+      rewrite (Mod.lookup_add_l Kt Ct fn (msk, body) WFT HKT) //=. }
+    iApply (isim_fsem_extend_ctx contextual Ks Kt Cs Ct); eauto.
+  Qed.
+
+End ISIM_EXTEND_CTX.
