theories/simulations/msim/ISimFrame.v
@@ -1,0 +1,72 @@
+From CRIS.common Require Import Common ConcRA StatePredicate.
+From CRIS.modules Require Import LMod Mod.
+From CRIS.simulations.msim Require Import MSim MSimFacts
+  MSimCommon ISim TacticsCommon ITactics.
+From iris.proofmode Require Import proofmode.
+
+Section ISIM_FRAME.
+  Context `{!crisG Γ Σ α β τ _S _I}.
+  Context `{!stateGS Σ}.
+
+  Lemma isim_ist_frame ctx Ist P Rs Rt RR fl_src fl_tgt
+      ps pt (i_s : itree crisE Rs) (i_t : itree crisE Rt) :
+    P ∗ isim ctx fl_src fl_tgt Ist ibot RR ps pt i_s i_t ⊢
+    isim ctx fl_src fl_tgt
+      (P ∗ Ist)%I ibot (λ x y, P ∗ RR x y) ps pt i_s i_t.
+  Proof using.
+    eapply entails_pointwise. intros res VALID H.
+    eapply isim_final.
+    eapply Own_split in H as
+      [rP [rSIM [EQ [HP HSIM]]]]; eauto.
+    eapply isim_init in HSIM; et.
+    gfinal. right.
+    eapply paco8_mon; [eapply msim_ist_frame|]; ss.
+    - ginit. eapply gpaco8_mon; eauto using iunlift_ibot.
+    - rewrite EQ Own_op HP. et.
+  Qed.
+
+  Local Lemma isim_fsem_frame ctx fl_src fl_tgt Ist P fs ft :
+    isim_fsem fl_src fl_tgt Ist ctx fs ft ⊢
+    isim_fsem fl_src fl_tgt (P ∗ Ist)%I ctx fs ft.
+  Proof.
+    rewrite /isim_fsem. iIntros "#FSIM !#" (arg) "[P IST] W".
+    iPoseProof ("FSIM" $! arg with "IST W") as "SIM".
+    iCombine "P SIM" as "SIM".
+    iPoseProof (isim_ist_frame with "SIM") as "SIM".
+    iApply (isim_mono ctx fl_src fl_tgt (P ∗ Ist)%I ibot false false
+      (λ x y, (P ∗ ist_with_eq Ist x y)%I)
+      (ist_with_eq (P ∗ Ist)%I) (fs arg) (ft arg)).
+    - iIntros (vsrc vtgt) "[P [-> IST]]".
+      iSplit; first done.
+      iSplitL "P"; done.
+    - done.
+  Qed.
+
+End ISIM_FRAME.
+
+Section ISIM_SIM_FUNS_FRAME.
+  Context `{!crisG Γ Σ α β τ _S _I}.
+
+  Lemma ISim_sim_funs_frame ctx Ks Kt Ist P Ms Mt :
+    ISim.sim_funs ctx Ks Kt Ist Ms Mt ⊢
+    ISim.sim_funs ctx Ks Kt
+      (λ STATE, (P STATE ∗ Ist STATE)%I) Ms Mt.
+  Proof.
+    rewrite /ISim.sim_funs. iIntros "SIM %WF".
+    iDestruct ("SIM" $! WF) as "[%PURE SIM]".
+    iSplit; first done.
+    iIntros (fn) "%IN".
+    iSpecialize ("SIM" $! fn with "[]"); first done.
+    rewrite /ISim.sim_fun.
+    iIntros (STATE).
+    iIntros "%WFS %WFT" (fs) "%LOOK".
+    iEval (rewrite /ISim.sim_fun) in "SIM".
+    iSpecialize ("SIM" $! STATE with "[] []"); [done|done|].
+    iSpecialize ("SIM" $! fs with "[]"); first done.
+    iDestruct "SIM" as (ft) "[%LOOKT FSIM]".
+    iExists ft. iSplit; first done.
+    iApply (@isim_fsem_frame Γ Σ α β _S _I STATE).
+    done.
+  Qed.
+
+End ISIM_SIM_FUNS_FRAME.
