theories/simulations/msim/ISimHorComp.v
@@ -1,0 +1,169 @@
+From CRIS.common Require Import Common ConcRA StatePredicate.
+From CRIS.modules Require Import Mod.
+From CRIS.simulations.msim Require Import MSimCommon ISim.
+From iris.proofmode Require Import proofmode.
+From stdpp Require Import base list.
+
+Local Lemma mod_add_scope_set `{Σ : GRA} (m1 m2 : Mod.t) :
+  (list_to_set (Mod.scopes (m1 ★ m2)) : gset string) =
+    list_to_set (Mod.scopes m1) ∪ list_to_set (Mod.scopes m2).
+Proof.
+  apply set_eq. intros scope.
+  rewrite elem_of_list_to_set elem_of_union /=.
+  rewrite sorting.merge_sort_Permutation elem_of_app.
+  by rewrite !elem_of_list_to_set.
+Qed.
+
+Local Lemma mod_add_scope_disjoint `{Σ : GRA} (m1 m2 : Mod.t)
+    (WF : Mod.wf (m1 ★ m2)) :
+  (list_to_set (Mod.scopes m1) : gset string) ##
+    list_to_set (Mod.scopes m2).
+Proof.
+  intros scope IN1 IN2.
+  rewrite !elem_of_list_to_set in IN1, IN2.
+  pose proof (Mod.wf_scopes _ WF) as ND.
+  rewrite /= sorting.merge_sort_Permutation NoDup_app in ND.
+  destruct ND as [_ [DISJ _]]. exact (DISJ scope IN1 IN2).
+Qed.
+
+Local Lemma state_slice_union_with_l
+    (S1 S2 : gset string) (m1 m2 : gmap key (option Any.t))
+    (SCOPED2 : set_map fst (dom m2) ⊆ S2) (DISJ : S1 ## S2) :
+  state_slice S1 (union_with uwnd m1 m2) = state_slice S1 m1.
+Proof.
+  apply map_eq. intros k. rewrite !state_slice_lookup.
+  destruct (decide (k.1 ∈ S1)) as [IN|NIN]; last done.
+  rewrite lookup_union_with.
+  destruct (m2 !! k) eqn:LOOK2; last by destruct (m1 !! k).
+  exfalso. apply elem_of_dom_2 in LOOK2.
+  apply (DISJ k.1 IN), SCOPED2.
+  apply elem_of_map. exists k. done.
+Qed.
+
+Local Lemma state_slice_union_with_r
+    (S1 S2 : gset string) (m1 m2 : gmap key (option Any.t))
+    (SCOPED1 : set_map fst (dom m1) ⊆ S1) (DISJ : S1 ## S2) :
+  state_slice S2 (union_with uwnd m1 m2) = state_slice S2 m2.
+Proof.
+  apply map_eq. intros k. rewrite !state_slice_lookup.
+  destruct (decide (k.1 ∈ S2)) as [IN|NIN]; last done.
+  rewrite lookup_union_with.
+  destruct (m1 !! k) eqn:LOOK1; last by destruct (m2 !! k).
+  exfalso. apply elem_of_dom_2 in LOOK1.
+  apply (DISJ k.1).
+  - apply SCOPED1, elem_of_map. exists k. done.
+  - exact IN.
+Qed.
+
+Section HORIZONTAL_COMPOSITION.
+
+  Context `{!crisG Γ Σ α β τ _S _I}.
+
+  Lemma add_init_ist
+    (Ms Mt Ns Nt : Mod.t)
+    (IstM IstN : stateGS Σ -> iProp Σ)
+    : ISim.init_ist Ms Mt IstM
+      ∗ ISim.init_ist Ns Nt IstN
+      ⊢ ISim.init_ist (Ms ★ Ns) (Mt ★ Nt) (fun STATE => IstM STATE ∗ IstN STATE).
+  Proof.
+    iIntros "[HM HN]". rewrite /ISim.init_ist.
+    iIntros (WF).
+    destruct (Mod.add_wf_inv Mt Nt WF) as
+      [WFMT [WFNT [FNSDISJ SCOPEND]]].
+    iDestruct ("HM" $! WFMT) as "[%SCPM HM]".
+    iDestruct ("HN" $! WFNT) as "[%SCPN HN]".
+    pose (SMs := (list_to_set (Mod.scopes Ms) : gset string)).
+    pose (SMt := (list_to_set (Mod.scopes Mt) : gset string)).
+    pose (SNs := (list_to_set (Mod.scopes Ns) : gset string)).
+    pose (SNt := (list_to_set (Mod.scopes Nt) : gset string)).
+    assert (TGT_DISJ : SMt ## SNt).
+    { subst SMt SNt. apply mod_add_scope_disjoint. exact WF. }
+    assert (MS_SUB : SMs ⊆ SMt).
+    { intros scope IN. rewrite /SMs elem_of_list_to_set in IN.
+      rewrite /SMt elem_of_list_to_set.
+      eapply elem_of_submseteq; eauto. }
+    assert (NS_SUB : SNs ⊆ SNt).
+    { intros scope IN. rewrite /SNs elem_of_list_to_set in IN.
+      rewrite /SNt elem_of_list_to_set.
+      eapply elem_of_submseteq; eauto. }
+    assert (SRC_DISJ : SMs ## SNs) by set_solver.
+    assert (SLICE_SRC_M :
+      state_slice SMs (Mod.initial_st (Ms ★ Ns)) =
+        state_slice SMs (Mod.initial_st Ms)).
+    { apply state_slice_union_with_l with (S2 := SNs).
+      - apply Mod.well_scoped_init.
+      - exact SRC_DISJ. }
+    assert (SLICE_SRC_N :
+      state_slice SNs (Mod.initial_st (Ms ★ Ns)) =
+        state_slice SNs (Mod.initial_st Ns)).
+    { apply state_slice_union_with_r with (S1 := SMs).
+      - apply Mod.well_scoped_init.
+      - exact SRC_DISJ. }
+    assert (SLICE_TGT_M :
+      state_slice SMt (Mod.initial_st (Mt ★ Nt)) =
+        state_slice SMt (Mod.initial_st Mt)).
+    { apply state_slice_union_with_l with (S2 := SNt).
+      - apply Mod.well_scoped_init.
+      - exact TGT_DISJ. }
+    assert (SLICE_TGT_N :
+      state_slice SNt (Mod.initial_st (Mt ★ Nt)) =
+        state_slice SNt (Mod.initial_st Nt)).
+    { apply state_slice_union_with_r with (S1 := SMt).
+      - apply Mod.well_scoped_init.
+      - exact TGT_DISJ. }
+    iSplit.
+    { iPureIntro. simpl. rewrite !sorting.merge_sort_Permutation.
+      eapply submseteq_app; eauto. }
+    iIntros (STATE) "SRC TGT".
+    iEval (rewrite (mod_add_scope_set Ms Ns)) in "SRC".
+    iEval (rewrite (mod_add_scope_set Mt Nt)) in "TGT".
+    iPoseProof (state_init_src_union SMs SNs
+      (Mod.initial_st (Ms ★ Ns)) SRC_DISJ with "SRC") as "[SRCM SRCN]".
+    iPoseProof (state_init_tgt_union SMt SNt
+      (Mod.initial_st (Mt ★ Nt)) TGT_DISJ with "TGT") as "[TGTM TGTN]".
+    iPoseProof (state_init_src_ext SMs (Mod.initial_st (Ms ★ Ns))
+      (Mod.initial_st Ms) SLICE_SRC_M with "SRCM") as "SRCM".
+    iPoseProof (state_init_src_ext SNs (Mod.initial_st (Ms ★ Ns))
+      (Mod.initial_st Ns) SLICE_SRC_N with "SRCN") as "SRCN".
+    iPoseProof (state_init_tgt_ext SMt (Mod.initial_st (Mt ★ Nt))
+      (Mod.initial_st Mt) SLICE_TGT_M with "TGTM") as "TGTM".
+    iPoseProof (state_init_tgt_ext SNt (Mod.initial_st (Mt ★ Nt))
+      (Mod.initial_st Nt) SLICE_TGT_N with "TGTN") as "TGTN".
+    iSplitL "HM SRCM TGTM".
+    - iApply ("HM" $! STATE with "SRCM TGTM").
+    - iApply ("HN" $! STATE with "SRCN TGTN").
+  Qed.
+
+  Lemma add_sim_funs
+    (ctx : contextuality)
+    (Ks Kt : Mod.t)
+    (Ist : stateGS Σ -> iProp Σ)
+    (Ms Mt Ns Nt : Mod.t)
+    : ISim.sim_funs ctx Ks Kt Ist Ms Mt
+      ∗ ISim.sim_funs ctx Ks Kt Ist Ns Nt
+      ⊢ ISim.sim_funs ctx Ks Kt Ist (Ms ★ Ns) (Mt ★ Nt).
+  Proof.
+    iIntros "[HM HN]". rewrite /ISim.sim_funs.
+    iIntros (WF).
+    destruct (Mod.add_wf_inv Mt Nt WF) as
+      [WFMT [WFNT [TGT_DISJ SCOPEND]]].
+    iDestruct ("HM" $! WFMT) as "[%PUREM SIMM]".
+    iDestruct ("HN" $! WFNT) as "[%PUREN SIMN]".
+    destruct PUREM as [SOMEM SUBM].
+    destruct PUREN as [SOMEN SUBN].
+    assert (SRC_DISJ : dom (Mod.fnsems Ms) ## dom (Mod.fnsems Ns))
+      by set_solver.
+    iSplit.
+    { iPureIntro.
+      split.
+      - eapply map_Forall_union_with; eauto.
+      - rewrite !Mod.dom_fnsems_add. set_solver.
+    }
+    iIntros (fn) "%IN".
+    rewrite Mod.dom_fnsems_add in IN.
+    set_unfold in IN. destruct IN as [IN|IN].
+    - iApply ("SIMM" $! fn). done.
+    - iApply ("SIMN" $! fn). done.
+  Qed.
+
+End HORIZONTAL_COMPOSITION.
