theories/simulations/msim/ISimRefl.v
@@ -1,0 +1,350 @@
+From CRIS.common Require Import Common ConcRA StatePredicate.
+From CRIS.modules Require Import Mod.
+From CRIS.simulations.msim Require Import MSimCommon ISim TacticsCommon ITactics.
+From iris.proofmode Require Import proofmode.
+From stdpp Require Import base list.
+
+Section STATE_EQ.
+  Context {Σ : GRA}.
+
+  Definition state_eq (S : gset string) (STATE : stateGS Σ) : iProp Σ :=
+    ∃ st_src st_tgt : gmap key (option Any.t),
+      ⌜state_slice S st_src = state_slice S st_tgt⌝ ∗
+      state_init_src S st_src STATE ∗ state_init_tgt S st_tgt STATE.
+
+  Definition IstEq (M : Mod.t) : stateGS Σ → iProp Σ :=
+    state_eq (list_to_set (Mod.scopes M)).
+
+  Lemma state_eq_acc `{STATE : !stateGS Σ} S k (IN : k.1 ∈ S) :
+    state_eq S STATE ⊢
+      ∃ ov, state_cell_src k ov ∗ state_cell_tgt k ov ∗
+        (∀ ov', ⌜state_cell_transition ov ov'⌝ -∗
+          state_cell_src k ov' ∗ state_cell_tgt k ov' -∗
+          state_eq S STATE).
+  Proof.
+    rewrite /state_eq /=. iIntros "EQ".
+    iDestruct "EQ" as (st_src st_tgt) "(%EQ & SRC & TGT)".
+    iPoseProof (state_init_src_acc S st_src k IN with "SRC") as
+      (ov_src) "(%Hsrc & SRC & CLOSESRC)".
+    iPoseProof (state_init_tgt_acc S st_tgt k IN with "TGT") as
+      (ov_tgt) "(%Htgt & TGT & CLOSETGT)".
+    assert (Hov : ov_src = ov_tgt).
+    { rewrite Hsrc Htgt.
+      pose proof (f_equal (fun st => st !! k) EQ) as EQk.
+      rewrite (state_slice_lookup_in S st_src k IN)
+        (state_slice_lookup_in S st_tgt k IN) in EQk.
+      exact EQk. }
+    clear Htgt. subst ov_tgt.
+    iExists ov_src. iFrame "SRC TGT".
+    iIntros (ov') "%TRANS [SRC TGT]".
+    iExists (set_state_cell k ov' st_src),
+      (set_state_cell k ov' st_tgt).
+    iSplit.
+    { iPureIntro.
+      by apply state_slice_set_state_cell_eq. }
+    iSplitL "SRC CLOSESRC".
+    - iApply ("CLOSESRC" $! ov' with "[] SRC"). done.
+    - iApply ("CLOSETGT" $! ov' with "[] TGT"). done.
+  Qed.
+
+  Lemma state_eq_put `{STATE : !stateGS Σ} S k v' (IN : k.1 ∈ S) :
+    state_eq S STATE ⊢
+      ∃ ov, state_cell_src k ov ∗ state_cell_tgt k ov ∗
+        ((k ↦src v' ∗ k ↦tgt v') -∗ state_eq S STATE).
+  Proof.
+    iIntros "EQ".
+    iPoseProof (state_eq_acc S k IN with "EQ") as
+      (ov) "(SRC & TGT & CLOSE)".
+    iExists ov. iFrame "SRC TGT". iIntros "[SRC TGT]".
+    iApply ("CLOSE" $! (Some v') with "[] [SRC TGT]").
+    - iPureIntro. right. done.
+    - rewrite /state_cell_src /state_cell_tgt /=. iFrame.
+  Qed.
+
+  Lemma state_eq_get `{STATE : !stateGS Σ} S k (IN : k.1 ∈ S) :
+    state_eq S STATE ⊢
+      ∃ ov, state_cell_src k ov ∗ state_cell_tgt k ov ∗
+        ((state_cell_src k ov ∗ state_cell_tgt k ov) -∗
+          state_eq S STATE).
+  Proof.
+    iIntros "EQ".
+    iPoseProof (state_eq_acc S k IN with "EQ") as
+      (ov) "(SRC & TGT & CLOSE)".
+    iExists ov. iFrame "SRC TGT". iIntros "ST".
+    iApply ("CLOSE" $! ov with "[] ST").
+    iPureIntro. left. done.
+  Qed.
+
+  Lemma state_eq_init `{STATE : !stateGS Σ} S st_src st_tgt
+      (EQ : state_slice S st_src = state_slice S st_tgt) :
+    state_init_src S st_src STATE -∗
+    state_init_tgt S st_tgt STATE -∗
+    state_eq S STATE.
+  Proof.
+    iIntros "SRC TGT". iExists st_src, st_tgt. iFrame. done.
+  Qed.
+
+  Lemma state_eq_init_same `{STATE : !stateGS Σ} S st :
+    state_init_src S st STATE -∗
+    state_init_tgt S st STATE -∗
+    state_eq S STATE.
+  Proof.
+    iApply state_eq_init. done.
+  Qed.
+End STATE_EQ.
+
+Section ISIM_REFL.
+  Context `{!crisG Γ Σ α β τ _S _I}.
+  Context `{STATE : !stateGS Σ}.
+
+  (* Reflexivity of the isim relation *)
+  Lemma isim_refl g ctx (Ist : iProp Σ) fl_src fl_tgt msk ps pt {R}
+      (it : itree crisE R) :
+    (∀ k v', msk _ (subevent _ (SPut k v')) = true →
+      Ist ⊢ ∃ ov, state_cell_src k ov ∗ state_cell_tgt k ov ∗
+        ((k ↦src v' ∗ k ↦tgt v') -∗ Ist)) →
+    (∀ k, msk _ (subevent _ (SGet k)) = true →
+      Ist ⊢ ∃ ov, state_cell_src k ov ∗ state_cell_tgt k ov ∗
+        ((state_cell_src k ov ∗ state_cell_tgt k ov) -∗ Ist)) →
+    Ist ⊢
+    isim ctx fl_src fl_tgt Ist g (ist_with_eq Ist) ps pt
+      (SB.sandbox msk it) (SB.sandbox msk it).
+  Proof using.
+    intros Hset Hget.
+    revert it. combine_quant ps. combine_quant pt.
+    eapply isim_coind. intros g0 _ CIH [pt [ps it]].
+    destruct_quant CIH. iIntros "IST /=".
+    assert (CASE := case_itrH it); des; subst.
+    - istep. iFrame. done.
+    - istep_s. istep_t. iby_coind CIH; eauto.
+    - cNormT; cNormS. des_if.
+      { istep_s. iforce_t; iFrame "ASM". cNormT. iby_coind CIH. eauto. }
+      { istep_s; ss. }
+    - cNormT; cNormS. des_if.
+      { istep_s. iforce_t; iFrame "ASM". cNormT. iby_coind CIH. eauto. }
+      { istep_s; ss. }
+    - cNormT; cNormS. des_if.
+      { istep_t. iforce_s; iFrame. cNormS. iby_coind CIH. eauto. }
+      { istep_s; ss. }
+    - depdes c.
+      { cNormT; cNormS. des_if.
+        { icall "IST" as (?) "IST"; et. iby_coind CIH; eauto. }
+        { isteps_s; ss. }
+      }
+      { cNormT; cNormS. des_if.
+        { istep. iby_coind CIH; done. }
+        { isteps_s. ss. }
+      }
+      { cNormS; cNormT. des_if.
+        { iyield "IST" "IST". iby_coind CIH. eauto. }
+        { isteps_s. ss. }
+      }
+      { cNormS; cNormT. des_if.
+        { istep. iby_coind CIH. eauto. }
+        { isteps_s. ss. }
+      }
+    - depdes s.
+      { cNormT; cNormS.
+        rewrite ?resum_to_subevent ?subevent_subevent.
+        specialize (Hset k v); destruct (msk _ _) eqn:Hmsk;
+          [cNormS; cNormT|istep_s; ss].
+        iPoseProof (Hset eq_refl with "IST") as
+          (ov) "(SRC & TGT & CLOSE)".
+        destruct ov as [v0|].
+        - iEval (rewrite /state_cell_src /state_cell_tgt /=) in "SRC TGT".
+          iApply isim_sput_src. iFrame "SRC". iIntros "SRC".
+          iApply isim_sput_tgt. iFrame "TGT". iIntros "TGT".
+          iby_coind CIH. iApply ("CLOSE" with "[$SRC $TGT]").
+        - iEval (rewrite /state_cell_src /state_cell_tgt /=) in "SRC TGT".
+          iApply isim_sput_src_uninit. iFrame "SRC". iIntros "SRC".
+          iApply isim_sput_tgt_uninit. iFrame "TGT". iIntros "TGT".
+          iby_coind CIH. iApply ("CLOSE" with "[$SRC $TGT]").
+      }
+      { cNormT; cNormS.
+        rewrite ?resum_to_subevent ?subevent_subevent.
+        specialize (Hget k); destruct (msk _ _) eqn:Hmsk;
+          [cNormS; cNormT|istep_s; ss].
+        iPoseProof (Hget eq_refl with "IST") as
+          (ov) "(SRC & TGT & CLOSE)".
+        destruct ov as [v|].
+        - iEval (rewrite /state_cell_src /state_cell_tgt /=) in "SRC TGT".
+          iApply isim_sget_src. iFrame "SRC". iIntros "SRC".
+          iApply isim_sget_tgt. iFrame "TGT". iIntros "TGT".
+          iby_coind CIH.
+          iApply ("CLOSE" with "[$SRC $TGT]").
+        - iEval (rewrite /state_cell_src /state_cell_tgt /=) in "SRC TGT".
+          iApply isim_sget_src_uninit. iFrame "SRC". iIntros "SRC".
+          iApply isim_sget_tgt_uninit. iFrame "TGT". iIntros "TGT".
+          iby_coind CIH.
+          iApply ("CLOSE" with "[$SRC $TGT]").
+      }
+    - destruct e.
+      + cNormT; cNormS. des_if; [cNormS; cNormT|istep_s; ss].
+        istep_t. iforce_s. cNormS; cNormT; iby_coind CIH; eauto.
+      + cNormT; cNormS. des_if; [cNormS; cNormT|istep_s; ss].
+        istep_s. iforce_t. cNormS; cNormT; iby_coind CIH; eauto.
+      + cNormT; cNormS. des_if; [cNormS; cNormT|istep_s; ss].
+        istep. cNormS; cNormT; iby_coind CIH; eauto.
+  Qed.
+
+  Lemma isim_reflL
+      (ctx : contextuality) (fl_src fl_tgt : gmap fname (option fbody))
+      (msk : emask) (EqL Ist : iProp Σ) itr :
+    (∀ k v', msk _ (subevent _ (SPut k v')) = true →
+      EqL ⊢ ∃ ov, state_cell_src k ov ∗ state_cell_tgt k ov ∗
+        ((k ↦src v' ∗ k ↦tgt v') -∗ EqL)) →
+    (∀ k, msk _ (subevent _ (SGet k)) = true →
+      EqL ⊢ ∃ ov, state_cell_src k ov ∗ state_cell_tgt k ov ∗
+        ((state_cell_src k ov ∗ state_cell_tgt k ov) -∗ EqL)) →
+    ⊢ isim_fsem fl_src fl_tgt (EqL ∗ Ist)%I ctx
+        (SB.sandbox_body (msk, itr)) (SB.sandbox_body (msk, itr)).
+  Proof using.
+    intros Hset Hget. rewrite /isim_fsem.
+    iIntros "!#" (arg) "[E I] _".
+    rewrite /SB.sandbox_body /=. iApply isim_refl.
+    - intros k v' Hmsk. iIntros "[E I]".
+      iPoseProof (Hset k v' Hmsk with "E") as
+        (ov) "(SRC & TGT & CLOSE)".
+      iExists ov. iFrame "SRC TGT". iIntros "[SRC TGT]".
+      iSplitR "I"; last done. iApply ("CLOSE" with "[$SRC $TGT]").
+    - intros k Hmsk. iIntros "[E I]".
+      iPoseProof (Hget k Hmsk with "E") as
+        (ov) "(SRC & TGT & CLOSE)".
+      iExists ov. iFrame "SRC TGT". iIntros "[SRC TGT]".
+      iSplitR "I"; last done. iApply ("CLOSE" with "[$SRC $TGT]").
+    - iFrame.
+  Qed.
+
+  Lemma isim_reflR
+      (ctx : contextuality) (fl_src fl_tgt : gmap fname (option fbody))
+      (msk : emask) (Ist EqR : iProp Σ) itr :
+    (∀ k v', msk _ (subevent _ (SPut k v')) = true →
+      EqR ⊢ ∃ ov, state_cell_src k ov ∗ state_cell_tgt k ov ∗
+        ((k ↦src v' ∗ k ↦tgt v') -∗ EqR)) →
+    (∀ k, msk _ (subevent _ (SGet k)) = true →
+      EqR ⊢ ∃ ov, state_cell_src k ov ∗ state_cell_tgt k ov ∗
+        ((state_cell_src k ov ∗ state_cell_tgt k ov) -∗ EqR)) →
+    ⊢ isim_fsem fl_src fl_tgt (Ist ∗ EqR)%I ctx
+        (SB.sandbox_body (msk, itr)) (SB.sandbox_body (msk, itr)).
+  Proof using.
+    intros Hset Hget. rewrite /isim_fsem.
+    iIntros "!#" (arg) "[I E] _".
+    rewrite /SB.sandbox_body /=. iApply isim_refl.
+    - intros k v' Hmsk. iIntros "[I E]".
+      iPoseProof (Hset k v' Hmsk with "E") as
+        (ov) "(SRC & TGT & CLOSE)".
+      iExists ov. iFrame "SRC TGT". iIntros "[SRC TGT]".
+      iSplitL "I"; first done. iApply ("CLOSE" with "[$SRC $TGT]").
+    - intros k Hmsk. iIntros "[I E]".
+      iPoseProof (Hget k Hmsk with "E") as
+        (ov) "(SRC & TGT & CLOSE)".
+      iExists ov. iFrame "SRC TGT". iIntros "[SRC TGT]".
+      iSplitL "I"; first done. iApply ("CLOSE" with "[$SRC $TGT]").
+    - iFrame.
+  Qed.
+
+End ISIM_REFL.
+
+Section ISIM_MODULE_REFL.
+  Context `{!crisG Γ Σ α β τ _S _I}.
+
+  Lemma ISim_init_ist_refl (M : Mod.t) :
+    ⊢ ISim.init_ist M M (IstEq M).
+  Proof.
+    rewrite /ISim.init_ist. iIntros (WF). iSplit.
+    { done. }
+    iIntros (STATE) "SRC TGT".
+    iApply (@state_eq_init_same Σ STATE (list_to_set (Mod.scopes M))
+      (Mod.initial_st M) with "SRC TGT").
+  Qed.
+
+  Lemma ISim_sim_funs_refl (ctx : contextuality) (M : Mod.t) :
+    ⊢ ISim.sim_funs ctx M M (IstEq M) M M.
+  Proof.
+    rewrite /ISim.sim_funs. iIntros (WF). iSplit.
+    { iPureIntro. split.
+      - apply WF.
+      - done. }
+    iIntros (fn) "%Hfn". rewrite /ISim.sim_fun.
+    iIntros (STATE).
+    iIntros "%WFS %WFT" (fs) "%Hfs".
+    rewrite lookup_fmap in Hfs.
+    destruct (Mod.fnsems M !! fn) as [[[fmsk fbdy]|]|] eqn:Hc; ss.
+    hexploit (Mod.well_scoped_fns M fn (fmsk, fbdy)).
+    { rewrite lookup_omap Hc //. }
+    intros [HPUT HGET].
+    clarify. iExists (SB.sandbox_body (fmsk, fbdy)).
+    iSplit; first by rewrite /sandbox_fnsemmap lookup_fmap Hc.
+    rewrite /isim_fsem. iIntros "!#" (arg) "IST _".
+    rewrite /SB.sandbox_body /=. iApply (@isim_refl Σ STATE).
+    - intros k v Hmsk. iApply (@state_eq_put Σ STATE).
+      rewrite elem_of_list_to_set. eapply HPUT. exact Hmsk.
+    - intros k Hmsk. iApply (@state_eq_get Σ STATE).
+      rewrite elem_of_list_to_set. eapply HGET. exact Hmsk.
+    - iFrame.
+  Qed.
+
+  Lemma ISim_refl (ctx : contextuality) (M : Mod.t) :
+    ⊢ ISim.t ctx M M (IstEq M).
+  Proof.
+    rewrite /ISim.t. iSplit.
+    - iApply ISim_init_ist_refl.
+    - iApply ISim_sim_funs_refl.
+  Qed.
+
+End ISIM_MODULE_REFL.
+
+Section STATE_EQ_RULES.
+
+  Context `{!crisG Γ Σ α β τ _S _I}.
+  Context `{STATE : !stateGS Σ}.
+
+  #[local] Set Implicit Arguments.
+
+  Lemma isim_sput_eq ctx fl_s fl_t S g {Rs Rt} RR ps pt k v' k_s k_t
+      (IN : k.1 ∈ S) :
+    state_eq S STATE ∗
+      (state_eq S STATE -∗
+        @isim Σ _ ctx fl_s fl_t (state_eq S STATE) g Rs Rt RR
+          true true (k_s tt) (k_t tt)) ⊢
+    @isim Σ _ ctx fl_s fl_t (state_eq S STATE) g Rs Rt RR ps pt
+      (trigger (SPut k v') >>= k_s) (trigger (SPut k v') >>= k_t).
+  Proof.
+    iIntros "[EQ SIM]".
+    iPoseProof (state_eq_put S k v' IN with "EQ") as
+      (ov) "(SRC & TGT & CLOSE)".
+    destruct ov as [v|].
+    - iEval (rewrite /state_cell_src /state_cell_tgt /=) in "SRC TGT".
+      iApply isim_sput_src. iFrame "SRC". iIntros "SRC".
+      iApply isim_sput_tgt. iFrame "TGT". iIntros "TGT".
+      iApply "SIM". iApply ("CLOSE" with "[$SRC $TGT]").
+    - iEval (rewrite /state_cell_src /state_cell_tgt /=) in "SRC TGT".
+      iApply isim_sput_src_uninit. iFrame "SRC". iIntros "SRC".
+      iApply isim_sput_tgt_uninit. iFrame "TGT". iIntros "TGT".
+      iApply "SIM". iApply ("CLOSE" with "[$SRC $TGT]").
+  Qed.
+
+  Lemma isim_sget_eq ctx fl_s fl_t S g {Rs Rt} RR ps pt k k_s k_t
+      (IN : k.1 ∈ S) :
+    state_eq S STATE ∗
+      (∀ v, state_eq S STATE -∗
+        @isim Σ _ ctx fl_s fl_t (state_eq S STATE) g Rs Rt RR
+          true true (k_s v) (k_t v)) ⊢
+    @isim Σ _ ctx fl_s fl_t (state_eq S STATE) g Rs Rt RR ps pt
+      (trigger (SGet k) >>= k_s) (trigger (SGet k) >>= k_t).
+  Proof.
+    iIntros "[EQ SIM]".
+    iPoseProof (state_eq_get S k IN with "EQ") as
+      (ov) "(SRC & TGT & CLOSE)".
+    destruct ov as [v|].
+    - iEval (rewrite /state_cell_src /state_cell_tgt /=) in "SRC TGT".
+      iApply isim_sget_src. iFrame "SRC". iIntros "SRC".
+      iApply isim_sget_tgt. iFrame "TGT". iIntros "TGT".
+      iApply ("SIM" $! v). iApply ("CLOSE" with "[$SRC $TGT]").
+    - iEval (rewrite /state_cell_src /state_cell_tgt /=) in "SRC TGT".
+      iApply isim_sget_src_uninit. iFrame "SRC". iIntros "SRC".
+      iApply isim_sget_tgt_uninit. iFrame "TGT". iIntros "TGT".
+      iApply ("SIM" $! (tt↑)). iApply ("CLOSE" with "[$SRC $TGT]").
+  Qed.
+
+End STATE_EQ_RULES.
